Paper

Haberl/Earley/Paper/Paper.thy
@@ -4,18 +4,117 @@ imports
   "Earley.EarleyWorklist"
   Sugar
 begin
+(* set_ItemList \<rightarrow> set_IL *)
+(* TODO: localize interpretation in EarleyWorklist *)
 declare [[show_question_marks=false]]
 declare [[names_short=true]]
 
-definition le_O :: "('a \<Rightarrow> nat) \<Rightarrow> ('a \<Rightarrow> nat) \<Rightarrow> ('a \<Rightarrow> bool) \<Rightarrow> bool"
-  ("(_/ \<le>O _/ IF _)" [50, 1000, 0] 0)
-where "(f \<le>O g IF Q) = (\<exists>c d. \<forall>x. Q x \<longrightarrow> f x \<le> c * g x + d)"
+type_synonym ('n,'a)item_list = "('n,'a)efficientItemList"
+translations (type) "('n,'a)item_list" <= (type) "('n,'a)efficientItemList"
 
-notation (latex) le_O ("(_/ \<le>\<^bsub>\<^latex>\<open>\\isaconst{\<close>O\<^latex>\<open>}\<close>\<^esub> _/ IF _)" [50, 1000, 0] 0)
-abbreviation le_O_True :: "('a \<Rightarrow> nat) \<Rightarrow> ('a \<Rightarrow> nat) \<Rightarrow> bool"
-   (infix "\<le>O" 50)  where "f \<le>O g \<equiv> (f \<le>O g IF (\<lambda>x. True))"
+lemma empty_froms_is_replicate: "empty_froms n = replicate (n+1) []"
+by(induction n) auto
 
-lemma le_O_trans: "f \<le>O g IF Q \<Longrightarrow> g \<le>O h IF Q \<Longrightarrow> f \<le>O h IF Q"
+(*TODO use in def of T_steps *)
+definition T_while_option2
+  :: "('a \<Rightarrow> bool) \<Rightarrow> ('a \<Rightarrow> 'a) \<Rightarrow> ('a \<Rightarrow> nat) \<Rightarrow> 'a \<times> nat \<Rightarrow> ('a \<times> nat) option" where
+"T_while_option2 b f T_f = while_option (\<lambda>(x,n). b x) (\<lambda>(x,n). (f x, n + T_f x))"
+
+definition T_while_option :: "('a \<Rightarrow> bool) \<Rightarrow> ('a \<Rightarrow> 'a) \<Rightarrow> ('a \<Rightarrow> nat) \<Rightarrow> 'a \<Rightarrow> nat" where
+"T_while_option b f T_f x = snd (the (T_while_option2 b f T_f (x,0)))"
+
+text \<open>Sanity check:\<close>
+
+(* TODO *)
+lemma T_while_option2_sanity:
+  "T_while_option2 b f tf (x,n0) = Some (y,n) \<Longrightarrow> while_option b f x = Some y"
+unfolding T_while_option2_def
+(*  while_option_rule[of ""]*)
+  oops
+
+definition le_O :: "('a \<Rightarrow> bool) \<Rightarrow> ('a \<Rightarrow> nat) \<Rightarrow> ('a \<Rightarrow> nat) \<Rightarrow> bool"
+where "(le_O Q f g) = (\<exists>c d. \<forall>x. Q x \<longrightarrow> f x \<le> c * g x + d)"
+
+abbreviation O_le :: "('a \<Rightarrow> nat) \<Rightarrow> ('a \<Rightarrow> nat) \<Rightarrow> ('a \<Rightarrow> bool) \<Rightarrow> bool"
+  ("(_/ \<le>O _/ IF _)" [50, 1000, 0] 0) where
+"O_le f g Q \<equiv> le_O Q f g"
+
+abbreviation O_le0 :: "('a \<Rightarrow> nat) \<Rightarrow> ('a \<Rightarrow> nat) \<Rightarrow> bool" (infix "\<le>O" 50) where
+"O_le0 f g \<equiv> O_le f g (\<lambda>x. True)"
+
+notation (le_O_no_IF output) "O_le" ("(_/ \<le>O/ _)" [50,50] 50)
+
+notation (latex) O_le ("(_/ \<le>\<^bsub>\<^latex>\<open>\\isaconst{\<close>O\<^latex>\<open>}\<close>\<^esub> _/ IF _)" [50, 1000, 0] 0)
+
+lemma standard_BigO_if_le_O:
+  fixes m :: "'a \<Rightarrow> nat"
+  assumes "O_le0 (f o m) (g o m)" "finite {n. g(n) = 0}" "surj m"
+  shows "\<exists>c. \<exists>n0. \<forall>n \<ge> n0. f n \<le> c * g n"
+proof -
+  from assms(1) obtain c d where cd: "\<And>x. f(m x) \<le> c * g(m x) + d" unfolding le_O_def by auto
+  from assms(2) obtain k where k: "\<forall>n \<ge> k. g n \<noteq> 0"
+    by (metis (mono_tags, lifting) finite_nat_set_iff_bounded linorder_neq_iff mem_Collect_eq
+        order_le_less_trans)
+  let ?n0 = "max k (Min (m ` UNIV))"
+  have n0: "\<forall>n \<ge> ?n0. g n \<noteq> 0" using k
+    using max.bounded_iff by blast
+  let ?c = "c+d"
+  have "f n \<le> ?c * g n" if asm: "n \<ge> ?n0" for n
+  proof -
+    obtain x where "m x = n" using \<open>surj m\<close> by (metis surj_def)
+    have "d * g n \<ge> d" using n0 asm by auto
+    thus ?thesis using n0 cd[of x] asm unfolding add_mult_distrib
+      by (metis add.commute \<open>m x = n\<close> add_le_cancel_right le_trans)
+  qed
+  thus ?thesis by blast
+qed
+
+(* SYNTAX *)
+definition BigO :: "('a \<Rightarrow> nat * nat * bool) \<Rightarrow> bool"
+  where "BigO fgp \<equiv> \<exists>c d. \<forall>x f g p. fgp x = (f,g,p) \<longrightarrow> p \<longrightarrow> f \<le> c*g + d"
+
+syntax
+  "_BigO" :: "pttrn \<Rightarrow> bool \<Rightarrow> bool"  (\<open>(\<open>indent=3 notation=\<open>binder BIGO\<close>\<close>BIGO _./ _)\<close> [0, 10] 10)
+syntax (latex)
+  "_BigO" :: "pttrn \<Rightarrow> bool \<Rightarrow> bool"  (\<open>(\<open>indent=3 notation=\<open>binder BIGO\<close>\<close>\<^latex>\<open>\isaconst{\<close>O\<^latex>\<open>}\<close> _./ _)\<close> [0, 10] 10)
+
+syntax_consts "_BigO" \<rightleftharpoons> BigO
+
+definition fake_imp :: "bool \<Rightarrow> bool \<Rightarrow> bool" where
+"fake_imp P1 P2 \<equiv> (P1 \<longrightarrow> P2)"
+
+notation (fake_imp output) fake_imp  (infixr \<open>\<longrightarrow>\<close> 25)
+notation (no_fake_imp output) fake_imp ("\<^latex>\<open>\\hide{\<close>_\<^latex>\<open>}\<close>_")
+
+translations "BIGO x. Q" \<rightharpoonup> "CONST BigO (\<lambda>x. Q)"
+translations "BIGO x. CONST fake_imp p (a \<le> b)" \<leftharpoondown> "CONST BigO (\<lambda>x. (a, b, p))"
+
+lemma BigO_iff_le_O: "BigO (\<lambda>x. (f x, g x, Q x)) = ((\<lambda>x. f x) \<le>O g IF Q)"
+by(auto simp: le_O_def BigO_def)
+
+lemma BigO_if_le_O: "(\<lambda>x. f x) \<le>O g IF Q \<Longrightarrow> BigO (\<lambda>x. (f x, g x, Q x))"
+by(auto simp: le_O_def BigO_def)
+
+lemma BigO_if_le_O2: "(\<lambda>(x,y). f x y) \<le>O (\<lambda>(x,y). g x y) IF (\<lambda>(x,y). Q x y)
+  \<Longrightarrow> BigO (\<lambda>(x,y). (f x y, g x y, Q x y))"
+  by(auto simp: le_O_def BigO_def)
+
+lemma BigO_if_le_O3: "(\<lambda>(x,y,z). f x y z) \<le>O (\<lambda>(x,y,z). g x y z) IF (\<lambda>(x,y,z). Q x y z)
+  \<Longrightarrow> BigO (\<lambda>(x,y,z). (f x y z, g x y z, Q x y z))"
+  by(auto simp: le_O_def BigO_def)
+
+lemma le_O_init: "(\<And>x. Q x \<Longrightarrow> f x \<le> g x) \<Longrightarrow> f \<le>O g IF Q"
+by (metis add.commute add_0 le_O_def nat_mult_1)
+
+lemma le_O_init2: "(\<And>x y. Q x y \<Longrightarrow> f x y \<le> g x y)
+ \<Longrightarrow> (\<lambda>(x,y). f x y) \<le>O (\<lambda>(x,y). g x y) IF (\<lambda>(x,y). Q x y)"
+  by (simp add: le_O_init split_def)
+
+lemma le_O_init3: "(\<And>x y z. Q x y z \<Longrightarrow> f x y z \<le> g x y z)
+ \<Longrightarrow> (\<lambda>(x,y,z). f x y z) \<le>O (\<lambda>(x,y,z). g x y z) IF (\<lambda>(x,y,z). Q x y z)"
+  by (simp add: le_O_init split_def)
+
+lemma le_O_trans[trans]: "f \<le>O g IF Q \<Longrightarrow> g \<le>O h IF Q \<Longrightarrow> f \<le>O h IF Q"
   apply(auto simp: le_O_def)
   apply(rename_tac cg ch dg dh)
 apply(rule_tac x="cg*ch" in exI)
@@ -26,7 +125,7 @@ apply(erule_tac x=x in allE)
   apply(simp add: algebra_simps)
   by (metis add_mono_thms_linordered_semiring(2) distrib_left dual_order.trans mult_le_mono2)
 
-lemma le_O_trans2: "f \<le>O g IF Q \<Longrightarrow> g \<le>O h \<Longrightarrow> f \<le>O h IF Q"
+lemma le_O_trans2[trans]: "f \<le>O g IF Q \<Longrightarrow> g \<le>O h \<Longrightarrow> f \<le>O h IF Q"
   by (metis le_O_def le_O_trans)
 
 lemma le_O_id: "f \<le>O f IF Q"
@@ -58,9 +157,31 @@ done
 corollary le_O_add1: "g \<le>O f IF Q \<Longrightarrow> h \<le>O f IF Q \<Longrightarrow> (\<lambda>x. g x + h x) \<le>O f IF Q"
   using le_O_add by fastforce
 
+corollary le_O_add2L: "f \<le>O f' IF Q \<Longrightarrow> (\<lambda>x. f x + g x) \<le>O (\<lambda>x. f' x + g x) IF Q"
+  by (simp add: le_O_add1 le_O_init le_O_trans)
+
+corollary le_O_add2R: "f \<le>O f' IF Q \<Longrightarrow> (\<lambda>x. g x + f x) \<le>O (\<lambda>x. g x + f' x) IF Q"
+  by (simp add: le_O_add1 le_O_init le_O_trans)
+                               
 corollary le_O_Suc1: "g \<le>O f IF Q \<Longrightarrow> (\<lambda>x. Suc(g x)) \<le>O f IF Q"
   using le_O_add1[where h = "\<lambda>x. 1", OF _ le_O_k]
   by (metis (no_types, lifting) ext Suc_eq_plus1)
+
+
+lemma le_O_diff: "g \<le>O f IF Q \<Longrightarrow> (\<lambda>x. g x - h x) \<le>O f IF Q"
+apply(auto simp add: le_O_def)
+subgoal for c d
+apply(rule_tac x="c" in exI)
+apply(rule_tac x="d" in exI)
+apply auto
+  done
+  done
+
+lemma le_O_add_R1: "g \<le>O f1 IF Q \<Longrightarrow> g \<le>O (\<lambda>x. f1 x + f2 x) IF Q"
+by (meson le_O_init le_O_trans nat_le_iff_add)
+
+lemma le_O_add_R2: "g \<le>O f2 IF Q \<Longrightarrow> g \<le>O (\<lambda>x. f1 x + f2 x) IF Q"
+by (meson le_O_init le_O_trans2 le_add2)
 
 lemma le_O_mult_k: "g \<le>O f IF Q \<Longrightarrow> (\<lambda>x. k * g x) \<le>O f IF Q"
 apply(auto simp add: le_O_def)
@@ -72,6 +193,64 @@ by (metis add_mult_distrib2 mult.assoc mult_le_mono2)
 corollary le_O_mult_k2: "g \<le>O f IF Q \<Longrightarrow> (\<lambda>x. g x * k) \<le>O f IF Q"
   by (simp add: ab_semigroup_mult_class.mult.commute le_O_mult_k)
 
+lemma le_O_mult: "g1 \<le>O f1 IF Q \<Longrightarrow> g2 \<le>O f2 IF Q \<Longrightarrow>
+ (\<lambda>x. g1 x * g2 x) \<le>O (\<lambda>x. f1 x * f2 x) IF (\<lambda>x. Q x \<and> f1 x > 0 \<and> f2 x > 0)"
+apply(auto simp add: le_O_def)
+subgoal for c1 c2 d1 d2
+apply(rule_tac x="c1*c2+c1*d2+c2*d1" in exI)
+apply(rule_tac x="d1*d2" in exI)
+apply auto
+subgoal for x
+apply(erule_tac x=x in allE)
+  apply(erule_tac x=x in allE)
+apply(simp add: algebra_simps)
+  apply(drule (1) mult_mono)
+    apply simp_all
+  apply(simp add: algebra_simps)
+  apply(subgoal_tac "c1 * (d2 * (f1 x * f2 x)) \<ge> c1 * (d2 * f1 x)")
+  apply(subgoal_tac "c2 * (d1 * (f1 x * f2 x)) \<ge> c2 * (d1 * f2 x)")
+  apply linarith
+  apply simp
+  apply simp
+done
+done
+  done
+
+lemma le_O_multR: assumes "\<And>x. Q x \<Longrightarrow> g' x > 0" shows "g \<le>O g' IF Q \<Longrightarrow>
+ (\<lambda>x. f x * g x) \<le>O (\<lambda>x. f x * g' x) IF Q"
+apply(auto simp add: le_O_def)
+subgoal for c d
+apply(rule_tac x="c+d" in exI)
+apply(rule_tac x="0" in exI)
+apply auto
+subgoal for x
+apply(erule_tac x=x in allE)
+apply(simp add: algebra_simps)
+  apply(subgoal_tac "d \<le> d * g' x")
+  apply linarith
+  using assms[of x] by simp
+  done
+done
+
+lemma le_O_multL: assumes "\<And>x. Q x \<Longrightarrow> g' x > 0" shows "g \<le>O g' IF Q \<Longrightarrow>
+ (\<lambda>x. g x * f x) \<le>O (\<lambda>x. g' x * f x) IF Q"
+  using le_O_multR
+  by (metis (no_types, lifting) ext Groups.ab_semigroup_mult_class.mult.commute assms)
+
+lemma le_O_add_mult1: assumes "\<And>x. Q x \<Longrightarrow> g x > 0"
+  shows "(\<lambda>x. f x * g x + f x) \<le>O (\<lambda>x. f x * g x) IF Q"
+  apply(rule le_O_trans[of _ _ "\<lambda>x. f x * (g x + 1)"])
+  apply(rule le_O_init)
+   apply(simp add: algebra_simps)
+  apply(rule le_O_multR)
+  apply (simp add: assms)
+  using le_O_add1 le_O_id le_O_k by blast
+
+lemma le_O_mult': "\<lbrakk> \<And>x. f1 x > 0; \<And>x. f2 x > 0; g1 \<le>O f1 IF Q; g2 \<le>O f2 IF Q \<rbrakk> \<Longrightarrow>
+ (\<lambda>x. g1 x * g2 x) \<le>O (\<lambda>x. f1 x * f2 x) IF Q"
+  using le_O_mult[of Q g1 f1 g2 f2]
+  by presburger
+
 lemma le_O_le_power: assumes "k \<le> l" shows "(\<lambda>n. (f n)^k) \<le>O (\<lambda>n. (f n)^l) IF Q"
   unfolding le_O_def [[metis_instantiate]]
   by (metis add.commute assms less_one linorder_not_le nat_mult_1 order_class.order_eq_iff
@@ -80,20 +259,57 @@ lemma le_O_le_power: assumes "k \<le> l" shows "(\<lambda>n. (f n)^k) \<le>O (\<
 lemma le_O_id_le_power: "1 \<le> l \<Longrightarrow> (\<lambda>x. m x) \<le>O (\<lambda>x. (m x)^l) IF Q"
 using le_O_le_power by fastforce
 
-lemma le_O_init: "(\<And>x. Q x \<Longrightarrow> f x \<le> g x) \<Longrightarrow> f \<le>O g IF Q"
-by (metis add.commute add_0 le_O_def nat_mult_1)
+lemmas le_O_Is = le_O_id le_O_k le_O_Suc1 le_O_add1 le_O_diff le_O_mult_k le_O_mult_k2 le_O_le_power le_O_id_le_power
 
-lemma le_O_init3: "(\<And>x y z. Q x y z \<Longrightarrow> f x y z \<le> g x y z)
- \<Longrightarrow> (\<lambda>(x,y,z). f x y z) \<le>O (\<lambda>(x,y,z). g x y z) IF (\<lambda>(x,y,z). Q x y z)"
-  by (simp add: le_O_init split_def)
+lemma le_O_sq_plus1: "(\<lambda>x. (f x + 1)^2) \<le>O (\<lambda>x. (f x)^2)"
+  apply(auto simp: le_O_def)
+apply(rule_tac x="2" in exI)
+  apply(rule_tac x="2" in exI)
+  apply(simp add: algebra_simps power2_eq_square)
+  by (metis mult.commute Nat.nat_arith.rule0 mult_0_right
+      mult_Suc_right mult_le_mono1 nle_le not_less_eq_eq)
 
-lemmas le_O_Is = le_O_k le_O_Suc1 le_O_add1 le_O_mult_k le_O_mult_k2 le_O_le_power le_O_id_le_power
+lemma le_O_sq_Suc: "(\<lambda>x. (Suc(f x))^2) \<le>O (\<lambda>x. (f x)^2)"
+unfolding Suc_eq_plus1 by(rule le_O_sq_plus1)
+
+lemma plus1_cube_bound: "((n::nat) + 1) ^ 3 \<le> 7 * n ^ 3 + 1"
+proof -
+  show ?thesis
+  proof (cases "n=0")
+    case True
+    then show ?thesis by simp
+  next
+    case False
+    have "n \<le> n^3" by (simp add: numeral_3_eq_3)
+    moreover have "n^2 \<le> n^3" by (simp add: numeral_3_eq_3 numeral_2_eq_2)
+    moreover have "((n::nat) + 1) ^ 3 = n^3 + 3*n^2 + 3*n + 1" by(simp add: algebra_simps numeral_eq_Suc)
+    ultimately show ?thesis by linarith
+  qed
+qed
+
+lemma le_O_cube_plus1: "(\<lambda>x. (f x + 1)^3) \<le>O (\<lambda>x. (f x)^3)"
+  apply(auto simp: le_O_def)
+apply(rule_tac x=7 in exI)
+  apply(rule_tac x=1 in exI)
+  apply rule
+  subgoal for x
+    using plus1_cube_bound[of "f x"]
+    by simp
+  done
+corollary le_O_cube_Suc: "(\<lambda>x. (Suc(f x))^3) \<le>O (\<lambda>x. (f x)^3)"
+unfolding Suc_eq_plus1 by(rule le_O_cube_plus1)
+
+lemma le_O_fstI: "f \<le>O g \<Longrightarrow> (\<lambda>p. f(fst p)) \<le>O (\<lambda>p. g(fst p))"
+by (simp add: le_O_def)
+
 
 lemma "(\<lambda>x. 6*x^3 + 3*x^2 + 7*x + 13) \<le>O (\<lambda>n. n^3) IF Q"
 by(simp add: le_O_Is)
 
 (* TODO Earley: get rid of next_sym = Some, use not is_final ?? *)
 (* in step_fun: rename it*)
+(* get rid of global variables P w S from instations *)
+(* rename P to Prods? *)
 (*
 abbreviation "iupdate xs i f \<equiv> xs[i := f(xs!i)]"
 notation iupdate ("_[[_ := _]]" [1000,0,0] 0)
@@ -134,6 +350,11 @@ notation union_LIL (infixl \<open>\<union>\<^bsub>\<^latex>\<open>\isaconst{\scr
 notation minus_LIL ("\<^latex>\<open>\\isaconst{\<close>diff\<^bsub>\<^latex>\<open>\\isaconst{\\scriptsize \<close>LIL\<^latex>\<open>}\<close>\<^esub>\<^latex>\<open>}\<close>")
 notation minus_IL (infixl \<open>-\<^bsub>\<^latex>\<open>\isaconst{\scriptsize \<close>IL\<^latex>\<open>}\<close>\<^esub>\<close> 65)
 
+notation T_isin (\<open>\<^latex>\<open>\isaconst{\<close>T'_isin\<^bsub>\<^latex>\<open>\isaconst{\scriptsize \<close>IL\<^latex>\<open>}\<close>\<^esub>\<^latex>\<open>}\<close>\<close>)
+notation T_insert  (infixr \<open>\<^latex>\<open>\isaconst{\<close>T'_\<^latex>\<open>}\<close>#\<^bsub>\<^latex>\<open>\isaconst{\scriptsize \<close>IL\<^latex>\<open>}\<close>\<^esub>\<close> 65)
+notation T_union_LIL (\<open>\<^latex>\<open>\isaconst{\<close>T'_\<^latex>\<open>}\<close>\<union>\<^bsub>\<^latex>\<open>\isaconst{\scriptsize \<close>IL\<^latex>\<open>}\<close>\<^esub>\<close>)
+notation T_minus_IL (\<open>\<^latex>\<open>\isaconst{\<close>T'_\<^latex>\<open>}\<close>-\<^bsub>\<^latex>\<open>\isaconst{\scriptsize \<close>IL\<^latex>\<open>}\<close>\<^esub>\<close>)
+
 lemma Close2L_Predict: "\<lbrakk> \<not> is_complete x; C' = insert_list x C \<rbrakk> \<Longrightarrow>
     Close2L Bs (x#B,C) (diff_list (union_list (Predict_L x (length Bs)) B) C', C')"
   using Close2L.Predict by blast
@@ -157,53 +378,277 @@ notation bins_L ("\<^latex>\<open>\\isaconst{\<close>bins\<^bsub>\<^latex>\<open
 end
 
 locale Earley_Gw_eps_T2 = Earley_Gw_eps_T where ps = ps for ps :: "('n,'a) prods" +
-  assumes dist_ps: "distinct ps"
-  assumes T_nth_IL: "T_nth_IL i = i+1"
+  assumes T_nth_IL: "T_nth_IL i = 1"
 begin
+
+notation T_nth_IL ("\<^latex>\<open>\\isaconst{\<close>T'_nth\<^bsub>\<^latex>\<open>\\isaconst{\\scriptsize \<close>IL\<^latex>\<open>}\<close>\<^esub>\<^latex>\<open>}\<close>")
 
 notation T_step_fun ("\<^latex>\<open>\\isaconst{\<close>T'_step2\<^bsub>\<^latex>\<open>\\isaconst{\\scriptsize \<close>IL\<^latex>\<open>}\<close>\<^esub>\<^latex>\<open>}\<close>")
 
-lemma T_step_fun_bound2:
-  "(\<lambda>(Bs,il1,il2). T_step_fun Bs (il1, il2)) \<le>O
-(\<lambda>(Bs,il1,il2). L * Suc K * Suc (length Bs) * (7 * T_nth_IL (length Bs) + 3* L * Suc K + 7 + 2 * (K + 2))
-    + 7 * T_nth_IL (length Bs) + 3 * Suc (length Bs) + 2* L * Suc K + 7 + Suc K)
-IF (\<lambda>(Bs,il1,il2). id(list il1 \<noteq> [] \<and> wf_bins1 (map set Bs) \<and>
-  (\<forall>i < length Bs. distinct (Bs ! i))) \<and> id(wf1_IL il1 (length Bs) \<and> inv_IL il1 \<and>
-  length (froms il1) = Suc (length Bs)) \<and> wf1_IL il2 (length Bs) \<and> inv_IL il2 \<and>
-  length (froms il2) = Suc (length Bs))" unfolding id_def
-  apply(rule le_O_init3)
-  apply(rule T_step_fun_bound)
-  using dist_ps apply blast+
-  done
+definition T_close2_IL ::
+  "('n, 'a) item list list \<Rightarrow> ('n, 'a) efficientItemList \<times> ('n, 'a) efficientItemList \<Rightarrow> nat" where
+"T_close2_IL Bs =
+  T_while_option (\<lambda>(il1,il2). list il1 \<noteq> []) (step_fun Bs) (T_step_fun Bs)"
+
+notation T_close2_IL ("\<^latex>\<open>\\isaconst{\<close>T'_close2\<^bsub>\<^latex>\<open>\\isaconst{\\scriptsize \<close>IL\<^latex>\<open>}\<close>\<^esub>\<^latex>\<open>}\<close>")
+
+lemma T_steps_eq_T_close2_IL:
+  "T_steps Bs = T_close2_IL Bs"
+unfolding T_close2_IL_def T_while_option_def T_while_option2_def T_steps.simps steps_time.simps
+by(simp add: split_def) 
+
+notation T_bins_L ("\<^latex>\<open>\\isaconst{\<close>T'_bins\<^bsub>\<^latex>\<open>\\isaconst{\\scriptsize \<close>IL\<^latex>\<open>}\<close>\<^esub>\<^latex>\<open>}\<close>")
+
+lemma le_O_add_k_L_iff: "((\<lambda>x. k + f x) \<le>O g IF Q) \<longleftrightarrow> (f \<le>O g IF Q)"
+by (metis (no_types, lifting) ext le_O_add1 le_O_add_R2 le_O_id le_O_k le_O_trans)
+
+lemma le_O_plus_k_R_iff[simp]: "(f \<le>O (\<lambda>x. k + g x) IF Q) \<longleftrightarrow> (f \<le>O g IF Q)"
+using le_O_add_k_L_iff le_O_id le_O_trans2 by blast
+
+lemma T_steps_le_O: "(\<lambda>(Bs,il1,il2). T_steps Bs (il1, il2)) \<le>O (\<lambda>(Bs,il1,il2). (length Bs)^2)
+  IF (\<lambda>(Bs,il1,il2). wf_bins1 (map set Bs) \<and> wf1_IL il1 (length Bs) \<and> wf1_IL il2 (length Bs)
+     \<and> inv_IL il1 \<and> inv_IL il2 \<and> (\<forall>i < length Bs. distinct (Bs ! i))
+     \<and> set_ItemList il1 \<inter> set_ItemList il2 = {}
+     \<and> length (froms il1) = Suc (length Bs) \<and> length (froms il2) = Suc (length Bs))" (is "?f \<le>O ?g IF ?Q")
+proof -
+  have 1: "?f \<le>O (\<lambda>(Bs,il1,il2). (L * Suc K * Suc (length Bs)) * (L * Suc K * Suc (length Bs) * (7 * 1 + 3 * L * Suc K + 7 + 2 * (K + 2))
+   + 7 * 1 + 3 * Suc (length Bs) + 2 * L * Suc K + 7 + Suc K)) IF ?Q"
+    by(rule le_O_init3, elim conjE, rule T_steps_bound[unfolded T_nth_IL])
+  also have 2: "\<dots> \<le>O (\<lambda>(Bs,il1,il2).
+ (L * Suc K) * (Suc (length Bs) *
+ (L * Suc K * Suc (length Bs) * (14 + 3 * L * Suc K + 2 * (K + 2))
+  + 3 * Suc (length Bs) + 2 * L * Suc K + 14 + Suc K)))"
+    unfolding split_def apply(rule le_O_init) by(simp add: algebra_simps)
+  also
+  have "\<dots> \<le>O (\<lambda>(Bs,il1,il2). Suc (length Bs) *
+ (L * Suc K * Suc (length Bs) * (14 + 3 * L * Suc K + 2 * (K + 2))
+  + 3 * Suc (length Bs) + 2 * L * Suc K + 14 + Suc K)) IF ?Q"
+    unfolding split_def by (rule le_O_mult_k[OF le_O_id])
+  also have "\<dots> \<le>O (\<lambda>(Bs,il1,il2). Suc (length Bs) *
+ (L * Suc K * Suc (length Bs) * (14 + 3 * L * Suc K + 2 * (K + 2))
+  + 3 * Suc (length Bs)))"
+    unfolding split_def apply(rule le_O_multR) apply simp
+    by(rule le_O_Is)+
+  also have "\<dots> \<le>O (\<lambda>(Bs,il1,il2). Suc (length Bs) * (L * Suc K * Suc (length Bs)
+  + 3 * Suc (length Bs)))"
+    unfolding split_def apply(rule le_O_multR) apply simp
+    apply(rule le_O_add2L)
+     apply (intro le_O_Is)
+    done
+  also have "\<dots> \<le>O (\<lambda>(Bs,il1,il2). (L * Suc K + 3) * (length Bs + 1)^2) IF ?Q"
+    unfolding split_def apply(rule le_O_init) by (simp add: algebra_simps power2_eq_square power3_eq_cube)
+  also have 1: "\<dots> \<le>O (\<lambda>(Bs,il1,il2). (length Bs + 1)^2)"
+    unfolding split_def
+    by(rule le_O_Is)+
+  also have 1: "\<dots> \<le>O ?g"
+    unfolding split_def using le_O_trans2[OF le_O_id le_O_fstI[OF le_O_sq_plus1]] .
+  finally show ?thesis .
+qed
+
+lemmas T_close2_IL_O = BigO_if_le_O3[OF T_steps_le_O[unfolded T_steps_eq_T_close2_IL]]
+
+
+lemma T_bins_IL_le_O: "T_bins_L \<le>O (\<lambda>k. k^3) IF (\<lambda>k. k \<le> length w)"
+proof -
+  note le_O_cube_SucSuc = le_O_trans[OF le_O_cube_Suc[of Suc] le_O_cube_Suc[of "\<lambda>x. x"]]
+  have "T_bins_L \<le>O (\<lambda>k. (k+2)^3 * ((Suc L * Suc K * Suc L * Suc K * (7 * T_nth_IL (Suc k) + 3* L * Suc K + 10 + 2 * (K + 2))) + (Suc L * Suc K * (2 * (K + 2) + 10 * T_nth_IL (Suc k) + 3* L * Suc K + 9 + Suc K)))) IF (\<lambda>k. k \<le> length w)"
+    by(rule le_O_init, rule T_bins_L_bound)
+  also have "\<dots> \<le>O (\<lambda>k. k^3)"
+    apply (simp add: split_def T_nth_IL le_O_Is algebra_simps flip: power3_eq_cube)
+    apply(rule le_O_Is le_O_cube_SucSuc)+
+    done
+  finally show ?thesis .
+qed
+
+lemmas T_bins_IL_O = BigO_if_le_O[OF T_bins_IL_le_O]
+
+
+lemma T_isin_le_O: "(\<lambda>(il,x). T_isin il x) \<le>O (\<lambda>(il,x). 1)
+  IF \<lambda>(il,x). inv_IL il \<and> wf1_IL il k \<and> from x < length (froms il)" (is "?f \<le>O ?g IF ?Q")
+proof -
+  have "?f \<le>O (\<lambda>(il,x). T_nth_IL (from x) + L * (Suc K) + 1) IF ?Q"
+    by(rule le_O_init2, elim conjE, rule T_isin_wf)
+  also have "\<dots> \<le>O (\<lambda>(il,x). 1) IF ?Q"
+    by(simp add: T_nth_IL split_def le_O_Is)
+  finally show ?thesis .
+qed
+
+lemmas T_isin_O = BigO_if_le_O2[OF T_isin_le_O]
+
+
+lemma T_insert_le_O: "(\<lambda>(x,il). T_insert x il) \<le>O (\<lambda>(x,il). 1)
+  IF \<lambda>(x,il). inv_IL il \<and> wf1_IL il k \<and> from x < length (froms il)" (is "?f \<le>O ?g IF ?Q")
+proof -
+  have "?f \<le>O (\<lambda>(x,il). 3 * T_nth_IL (from x) + L * (Suc K) + 1) IF ?Q"
+    by(rule le_O_init2, elim conjE, rule T_insert_less)
+  also have "\<dots> \<le>O (\<lambda>(x,il). 1) IF ?Q"
+    by(simp add: T_nth_IL split_def le_O_Is)
+  finally show ?thesis .
+qed
+
+lemmas T_insert_O = BigO_if_le_O2[OF T_insert_le_O]
+
+
+lemma T_step_fun_bound: assumes "(list il1) \<noteq> []" "wf_bins1 (map set Bs)" "\<forall>i < length Bs. distinct (Bs ! i)" "wf1_IL il1 (length Bs)" "inv_IL il1" "length (froms il1) = Suc (length Bs)"
+  "wf1_IL il2 (length Bs)" "inv_IL il2" "length (froms il2) = Suc (length Bs)"
+shows "T_step_fun Bs (il1, il2) 
+    \<le> L * Suc K * Suc (length Bs) * (7 * T_nth_IL (length Bs) + 3* L * Suc K + 7 + 2 * (K + 2))
+    + id(7 * T_nth_IL (length Bs) + 3 * Suc (length Bs) + 2* L * Suc K + 7 + Suc K)"
+unfolding id_def using T_step_fun_bound[OF assms] by linarith
 
 lemma aux2: "(n::nat)*(n*m) = n^2 * m"
   by(simp add: power2_eq_square)
 
-lemma T_step_fun_bound3: "(\<lambda>(Bs,il\<^sub>1,il\<^sub>2).
-  L * Suc K * Suc (length Bs) * (7 * T_nth_IL (length Bs) + 3* L * Suc K + 7 + 2 * (K + 2))
-+ 7 * T_nth_IL (length Bs) + 3 * Suc (length Bs) + 2* L * Suc K + 7 + Suc K) \<le>O
-  (\<lambda>(Bs,il1,il2). (length Bs)^2)"
-  unfolding split_def T_nth_IL
-  by (simp add: le_O_Is algebra_simps aux2 flip: power2_eq_square)
+lemma T_step_fun_bound_le_O: "(\<lambda>(Bs,il1,il2). T_step_fun Bs (il1, il2)) \<le>O (\<lambda>(Bs,il1,il2). (length Bs))
+  IF (\<lambda>(Bs,il1,il2). list il1 \<noteq> [] \<and> wf_bins1 (map set Bs) \<and>
+  (\<forall>i < length Bs. distinct (Bs ! i)) \<and> wf1_IL il1 (length Bs) \<and> inv_IL il1 \<and>
+  length (froms il1) = Suc (length Bs) \<and> wf1_IL il2 (length Bs) \<and> inv_IL il2 \<and>
+  length (froms il2) = Suc (length Bs))" (is "?f \<le>O ?g IF ?Q")
+proof -
+  have "?f \<le>O (\<lambda>(Bs,il1,il2).
+    L * Suc K * Suc (length Bs) * (7 * T_nth_IL (length Bs) + 3* L * Suc K + 7 + 2 * (K + 2))
+    + (7 * T_nth_IL (length Bs) + 3 * Suc (length Bs) + 2* L * Suc K + 7 + Suc K)) IF ?Q"
+    by(rule le_O_init3, elim conjE, rule T_step_fun_bound[unfolded id_def])
+  also have "\<dots> \<le>O ?g"
+    by (simp add: split_def T_nth_IL le_O_Is algebra_simps aux2 flip: power2_eq_square)
+  finally show ?thesis .
+qed
 
-lemmas T_step_fun_bound4 = le_O_trans2[OF T_step_fun_bound2 T_step_fun_bound3]
+lemmas T_step_fun_bound_O = BigO_if_le_O3[OF T_step_fun_bound_le_O]
+
+definition "T_union_LIL_wf_P \<equiv>
+  \<lambda>(as,il). inv_IL il \<and> wf1_IL il (length (froms il) - 1) \<and> wf_bin1 (set as) (length (froms il) - 1) 
+    \<and> (\<forall>a\<in>set as. from a < length (froms il))"
+
+lemma T_union_LIL_wf:
+ "(\<lambda>(as,il). T_union_LIL as il) \<le>O (\<lambda>(as,il). (length as) * (3 * T_nth_IL (length (froms il) - 1) + L * (Suc K) + 2) + 1)
+  IF T_union_LIL_wf_P"
+  unfolding T_union_LIL_wf_P_def
+  apply(rule le_O_init2)
+  apply(rule T_union_LIL_wf)
+  apply blast+
+  done
+
+lemma le_O_if_le2: "(\<And>x y. f x y \<le> f' x y) \<Longrightarrow> (\<lambda>(x,y). f x y) \<le>O (\<lambda>(x,y). f' x y)"
+  apply(auto simp add: le_O_def)
+  by (metis mult_1 trans_le_add1)
+
+lemma T_union_LIL_wf2:
+ "(\<lambda>(as,il). length as * (3 * T_nth_IL (length (froms il) - 1) + L * (Suc K) + 2) + 1)
+ \<le>O (\<lambda>(as,il). 3 * (length as * (1 + L * (Suc K) + 2)) + 1) IF T_union_LIL_wf_P"
+  unfolding T_nth_IL split_def
+  apply(rule le_O_init)
+  by (simp add: algebra_simps)
+
+lemma T_union_LIL_wf3:
+ "(\<lambda>(as,il). 3 * (length as * (1 + L * (Suc K) + 2)) + 1) \<le>O
+  (\<lambda>(as,il). length as * (1 + L * (Suc K) + 2)) IF T_union_LIL_wf_P"
+  unfolding split_def
+  by(rule le_O_Is)+
+
+lemma T_union_LIL_wf4:
+ "(\<lambda>(as,il). length as * (1 + L * (Suc K) + 2)) \<le>O
+  (\<lambda>(as,il). length as) IF T_union_LIL_wf_P"
+  unfolding split_def
+  by(simp add: split_def T_union_LIL_wf_P_def le_O_Is)
+(*  using EarleyWorklist.inv_IL.elims(2) apply fastforce
+  by(rule le_O_Is)+*)
+
+lemmas T_union_LIL_wf5=  BigO_if_le_O2[OF
+  le_O_trans[OF le_O_trans[OF le_O_trans[OF
+    T_union_LIL_wf T_union_LIL_wf2] T_union_LIL_wf3] T_union_LIL_wf4, unfolded T_union_LIL_wf_P_def]]
+
+definition "T_minus_IL_wf_P \<equiv> \<lambda>(il1,il2).
+  wf1_IL il1 (length (froms il1) - 1) \<and> inv_IL il1 \<and> inv_IL il2 \<and> wf1_IL il2 (length (froms il1) - 1)
+  \<and> length (froms il2) \<ge> length (froms il1)"
+
+lemma T_minus_IL_wf:
+  "(\<lambda>(il1,il2). T_minus_IL il1 il2) \<le>O (\<lambda>(il1,il2). (length (list il1)) * (4 * T_nth_IL (length (froms il1) - 1) + 2*L * (Suc K) + 4) + (length (froms il1) - 1) + 3 + length (list il1) + length (froms il1))
+  IF T_minus_IL_wf_P"
+  unfolding T_minus_IL_wf_P_def
+  apply(rule le_O_init2)
+  apply(rule T_minus_IL_wf)
+  apply blast+         
+  done
+
+lemma T_minus_IL_wf2:
+  "(\<lambda>(il1,il2). (length (list il1)) * (4 * T_nth_IL (length (froms il1) - 1) + 2*L * (Suc K) + 4) + (length (froms il1) - 1) + 3 + length (list il1) + length (froms il1))
+  \<le>O (\<lambda>(il1,il2). 4 * (length (list il1) * (2*L * (Suc K) + 4)) + 2*length (froms il1) + 3)
+  IF T_minus_IL_wf_P"
+  unfolding T_nth_IL split_def
+  apply(rule le_O_init)
+  by (simp add: algebra_simps)
+
+lemma le_O_add_k_L: "f \<le>O g IF Q \<Longrightarrow> (\<lambda>x. f x + k) \<le>O g IF Q"
+by (simp add: le_O_add1 le_O_k)
+
+lemma T_minus_IL_wf3:
+ "(\<lambda>(il1,il2). 4 * (length (list il1) * (2*L * (Suc K) + 4)) + 2*length (froms il1) + 3)
+ \<le>O (\<lambda>(il1,il2). length (list il1) + length (froms il1))
+  IF T_minus_IL_wf_P"
+  unfolding split_def
+  apply(rule le_O_Is)
+  apply(rule le_O_add1)
+  apply(rule le_O_add_R1)
+     apply(rule le_O_Is)
+(*     apply(rule le_O_multR)
+  apply(simp add: split_def T_minus_IL_wf_P_def)
+  using EarleyWorklist.inv_IL.elims(2) apply fastforce*)
+  apply(rule le_O_Is)
+  apply(rule le_O_Is)
+  apply(rule le_O_add_R2)
+  apply(rule le_O_Is)+
+  done
+(*
+lemma T_minus_IL_wf4:
+ "(\<lambda>(il1,il2). length (list il1) * length (froms il1) + length (froms il1))
+ \<le>O (\<lambda>(il1,il2). (length (list il1) + 1) * length (froms il1))
+  IF T_minus_IL_wf_P"
+  unfolding split_def
+  apply(rule le_O_init)
+  by (simp add: algebra_simps)
+*)
+lemmas T_minus_IL_wf5 =  BigO_if_le_O2[OF
+  (*le_O_trans[OF*) le_O_trans[OF le_O_trans[OF
+    T_minus_IL_wf T_minus_IL_wf2] T_minus_IL_wf3(*] T_minus_IL_wf4*), unfolded T_minus_IL_wf_P_def]]
 
 end
 
 (*>*)
 
 text\<open>
-
-\section{Introduction}
-
 \section{Isabelle Notation} \label{sec:isabelle}
 
-@{term "xs ! n"}
+The notation \<open>t :: \<tau>\<close> means that term \<open>t\<close> has type
+\<open>\<tau>\<close>. Basic types include @{typ bool} and @{typ nat}, while type variables are written @{typ 'a}, @{typ 'b} etc.
+Most type constructors are written postfix, such as @{typ "'a set"} and  @{typ "'a list"}, and the function
+space arrow is \<open>\<Rightarrow>\<close>.
+The image of function \<open>f\<close> over set \<open>M\<close> is denoted by @{prop "f ` A = {b. \<exists>a\<in>A. f a = b}"}.
+%Function update {term "f(a := b)"} is short for @{thm (rhs) fun_upd_def}.
 
-where @{prop "f ` A = {b. \<exists>a\<in>A. f a = b}"}.
+Functions @{const fst} and @{const snd} return the first and second components of a pair.
 
-@{const the}
+Lists are constructed from the empty list @{term "[]"} using the infix cons-operator @{term "(#)"}.
+The operator @{term "(@)"} appends two lists, @{term "length xs"} denotes the length of @{term xs},
+@{const set} converts a list to a set,
+@{term "xs!n"} returns the \<open>n\<close>-th element of the list \<open>xs\<close> (starting with @{prop "n=(0::nat)"})
+and @{term "xs[n := x]"} is \<open>xs\<close> with @{term "xs!n"} replaced by \<open>x\<close>.
 
+Algebraic data types are defined using the \isakeyword{datatype} keyword.
+The @{type option} type is predefined
+\begin{quote}
+@{datatype option}
+\end{quote}
+with the function @{thm Option.option.sel[of x]}.
+
+The notation \mbox{\<open>\<lbrakk>A\<^sub>1, \<dots>, A\<^sub>n\<rbrakk> \<Longrightarrow> B\<close>} denotes an implication with premises \<open>A\<^sub>1\<close>, \ldots, \<open>A\<^sub>n\<close> and conclusion \<open>B\<close>.
+Sometimes we use the inference rule presentation
+\begin{quote}
+\inferrule{\<open>A\<^sub>1\<close> \\ \ldots \\ \<open>A\<^sub>n\<close>}{B}
+\end{quote}
+
+
+Equality on type @{type bool} denotes logical equivalence.
 
 \subsection{Context-Free Grammars}
 
@@ -212,8 +657,8 @@ All our types are parameterized by type variables \<open>'n\<close> and \<open>'
 \begin{quote}
 @{datatype sym}
 \end{quote}
-Variable convention:
-% \<open>a, b, c :: 't\<close>, \<open>A, B, C :: 'n\<close> and  \<open>x, y, z :: ('n,'t) sym\<close>.
+Variable convention: \<open>A, B, C :: 'n\<close>.
+% \<open>a, b, c :: 't\<close>,  and  \<open>x, y, z :: ('n,'t) sym\<close>.
 For compactness we sometimes drop the \<open>'n\<close> and \<open>'t\<close> parameters,
 e.g.\ we write \<open>sym\<close> instead of \<open>('n,'t)sym\<close>.
 
@@ -227,7 +672,7 @@ We use the following abbreviations:
 %\<open>w :: 't list\<close>; lists over terminal symbols are called \concept{terminal words};
 %\<open>\<alpha>, \<beta>, \<gamma> :: syms\<close>; elements of type @{type syms} are called \concept{sentential forms}.
 
-Our theory is primarily based on sets of productions rather than grammars:
+Our work is primarily based on sets of productions rather than grammars:
 the start symbol is irrelevant most of the time.
 \emph{For succinctness, we use \concept{grammar} to refer to a set (or list) of productions.}
 Moreover, we only restrict to finite sets of productions when necessary.
@@ -243,17 +688,19 @@ The language of some nonterminal \<open>A\<close> generated by \<open>P\<close> 
 \begin{quote}
 @{thm Lang_def}
 \end{quote}
-\<close>
-
-text (in Earley_Gw_eps)\<open>
+\<close>text (in Earley_Gw_eps)\<open>
 \section{The Story so far}
 
-\cite{NipkowR-CBJ24}
+This paper is a continuation of the work by Nipkow and Rau \cite{NipkowR-CBJ24}.
+In this section few summarize the contents of the latter paper, which is a refinement
+of an initial inductive definition, via the standard definition to something resembling
+a worklist algorithm, but still as an inductive definition.
 
 \subsection{Inductive Definition of Earley's Item Sets} \label{sec:Earley}
+\label{sec:EarleyInductive}
 
 An Earley recognizer decides if some word is in the language described by a grammar
-by generating a set of so-called \emph{items} (\emph{states} in \cite{Earley} and \cite{NipkowR-CBJ24})
+by generating a set of so-called \emph{items} (also called \emph{states} in the literature)
 and checking if it contains a \emph{final} item.
 In the sequel, we fix the following ``global variables'':
 \begin{itemize}
@@ -263,9 +710,9 @@ In the sequel, we fix the following ``global variables'':
 \end{itemize}
 
 An item is a triple @{term "Item r d i"}
-where \<open>r = (A, \<alpha>)\<close> is a production from \<open>P\<close>, \<open>d\<close> is a natural number such that@{prop "d \<le> length \<alpha>"},
+where \<open>r = (A, \<alpha>)\<close> is a production from \<open>P\<close>, \<open>d\<close> is a natural number such that @{prop "d \<le> length \<alpha>"},
 indicating how far the algorithm has recognized \<open>\<alpha>\<close>,
-and \<open>i\<close> is a natural number representing the start index of the subword of \<open>w\<close>
+and \<open>i\<close> is a natural number representing the start index of the subword of @{term w}
 recognized by this item. The three projection functions are
 @{const prod}, @{const dot} and @{const from}. We use the letters \<open>x\<close> and \<open>y\<close> for items.
 
@@ -290,7 +737,7 @@ Note that @{prop "next_sym x s"} implies @{prop "\<not> is_complete x"}.
 Next we give an abstract inductive definition of @{const Earley}, a set
 of pairs @{term "(x,j)"} of items and an index. However, it is more intuitive
 to present it as an inductive definition of indexed item sets: we write
-\mbox{@{prop "x \<in> \<S> j"}} instead of @{term "(x,j)"} \<open>\<in> Earley\<close>.
+\mbox{@{prop "x \<in> \<S> j"}} instead of @{prop "(x,j)\<in> Earley"}.
 In the indexed presentation, we define item sets
 \mbox{@{term "\<S> j"}}, @{prop \<open>j \<le> |w|\<close>}, that depend on each other. However, the dependence is in
 one direction only: later sets depend on earlier ones, not the other way around.
@@ -301,7 +748,7 @@ The intuitive meaning of @{prop "Item r d i \<in> \<S> j"} is that the subword
 @{term "slice i j w"} (which stands for @{term "drop i (take j w)"}) has been recognized.
 We call \<open>i\<close> the \emph{start index} and \<open>j\<close> the \emph{end index} (which is excluded).
 
-The four defining rules are: the initial set of items, and one rule for each of the core operations that
+The four defining rules are: one rule for the initial set of items, and one rule for each of the core operations that
 expand the set of items: scanning, prediction, and completion.
 \begin{quote}
 {\sc Init}: @{thm [mode=Rule] Earley.Init[simplified Earley_eq_\<S>]} \quad where
@@ -358,10 +805,10 @@ The standard definition of Earley's algorithm
 generates each @{term "\<S> j"} completely before moving on to @{term "\<S> (j+1)"}.
 This sequential strategy works because elements of @{term "\<S> j"}
 do not depend on @{term "\<S> k"} where \<open>j < k\<close>.
-Therefore Earley \cite{Earley} starts with
+Therefore Earley \cite{Earley-CACM} starts with
 a more algorithmic formulation. The sets @{term "\<S> 0"}, @{term "\<S> 1"}, \dots, @{term "\<S> (length w)"}
 are generated in that order. We follow Jones and define a sequence of \emph{bins} (= item sets),
-where the \<open>i\<close>th bin is meant to hold @{term "\<S> i"}.
+where the \<open>i\<close>-th bin is meant to hold @{term "\<S> i"}.
 Function @{const bins} recursively computes the list of bins
 \begin{quote}
 %{const_typ "bins::bool"}\smallskip\\
@@ -393,7 +840,7 @@ In the end we proved the following correctness theorem:
 \subsection{Epsilon-free Closure}
 
 To simplify the computation of @{const Close}, we follow Jones and assume that @{const P}
-is epsilon-free in the rest of the paper, i.e. there is no production in @{const P} with an empty @{const rhs}.
+is epsilon-free in the rest of the paper, i.e.\ there is no production in @{const P} with an empty @{const rhs}.
 In that case, in the completion rule for @{const Close},
 @{prop "x \<in> mbox((Bs @ [Close Bs B])) ! from y"} can be simplified to
 @{prop "x \<in> Bs ! from y"}. Formally, we define a variant @{const Close1} of @{const Close}
@@ -446,38 +893,8 @@ The proof is by induction on a suitable wellfounded relation (that is based on t
 Although it is not obvious, there is a unique \<open>C'\<close> such that @{prop "Bs \<turnstile> (B, C) \<rightarrow>* ({}, C')"},
 i.e.\ the result of @{const close2} is independent of which result \<open>SOME\<close> chooses.
 
-As for @{const Close} and @{const Close1}, we can also prove the equivalence of @{const Close1} and @{const close2}:
-\begin{quote}
-@{thm close2_eq_Close1}
-\end{quote}
-
-We will sketch the proof because it is omitted in \cite{NipkowR-CBJ24}.
-All proofs are by obvious inductions.
-
-The following lemmas are generally useful:
-\begin{quote}
-@{thm Close2_steps_disj}\\
-@{thm Close2_steps_incr}
-\end{quote}
-
-Soundness (@{thm Close2_steps_subset_Close1'}) follows in two obvious steps:
-\begin{quote}
-@{thm Close2_step_subset_Close1}\\
-@{thm Close2_steps_subset_Close1}
-\end{quote}
-
-Completeness is a bit trickier. The key lemma says that in an \<open>\<rightarrow>\<close> sequence. where an element \<open>x\<close>
-starts in \<open>B\<close> and ends up in \<open>C'\<close>, there is a \<open>\<rightarrow>\<close> step where that transition takes place.
-Completeness can be proved from this lemma.
-\begin{quote}
-@{thm [break,margin=75] (sub) Close2_steps_subdivide}\smallskip\\
-@{thm Close2_sim_Close1}
-\end{quote}
-
-Altogether this yields the desired
-\begin{quote}
-@{thm Close2_eq_Close1}
-\end{quote}
+As for @{const Close} and @{const Close1}, we can also prove the equivalence of @{const Close1} and @{const close2}.
+This is relegated to Section \ref{sec:close2_eq_Close1}.
 
 Of course we still need to show termination of \<open>\<rightarrow>\<close>.
 This follows because the set of well-formed items (let us call it \<open>I\<close>) is finite,
@@ -488,20 +905,53 @@ which implies termination.
 By induction on this wellfounded relation it follows that eventually @{prop "B={}"}
 because if not, either prediction or completion applies.
 
-
-TODO Get rid of this:?
-
 Finally we can replace @{const Close} by @{const close2} in the definition of @{const bins}
 and obtain (by proof)
 \begin{quote}
 @{thm (concl) bins0_close2}\\
 @{thm (concl) binsSuc_close2}
 \end{quote}
-where we need to assume that @{prop "k < length w"}. This assumption does no harm
-because by definition of @{const accepted}, we only need to compute the bins up to @{term "length w"}.
 
 Of course, we have not yet arrived at an executable formulation because of the presence of \<open>SOME\<close>
 in @{const close2}.
+
+
+\subsection{Equivalence of @{const close2} and @{const Close1}}
+\label{sec:close2_eq_Close1}
+
+\begin{quote}
+@{thm close2_eq_Close1}
+\end{quote}
+
+We will sketch the proof because it is omitted in \cite{NipkowR-CBJ24}.
+All proofs are by obvious inductions.
+
+The following lemmas are generally useful:
+\begin{quote}
+@{thm Close2_steps_disj}\medskip\\
+@{thm Close2_steps_incr}
+\end{quote}
+
+Soundness (@{thm Close2_steps_subset_Close1'}) follows in two obvious steps:
+\begin{quote}
+@{thm Close2_step_subset_Close1}\medskip\\
+@{thm Close2_steps_subset_Close1}
+\end{quote}
+
+Completeness is a bit trickier. The key lemma says that in an \<open>\<rightarrow>\<close> sequence. where an element \<open>x\<close>
+starts in \<open>B\<close> and ends up in \<open>C'\<close>, there is a \<open>\<rightarrow>\<close> step where that transition takes place.
+\begin{quote}
+@{thm [break,margin=75] (sub) Close2_steps_subdivide}
+\end{quote}
+Completeness can be proved from this lemma.
+\begin{quote}
+@{thm Close2_sim_Close1}
+\end{quote}
+
+Altogether this yields the desired
+\begin{quote}
+@{thm Close2_eq_Close1}
+\end{quote}
 
 
 \section{Refinement}
@@ -529,11 +979,12 @@ and \<open>Bs\<close> is a list of item lists:
 \end{quote}
 where
 \begin{quote}
-@{thm Predict_L_def}\\
+@{thm Predict_L_def}\medskip
+
 @{thm [break] Complete_L_def}
 \end{quote}
-and @{const insert_list}, @{const union_list} and @{const diff_list} implement the corresponding
-set functions on lists. They are defined in Appendix~\ref{SetByList}. We have also replaced
+The binary operations @{const insert_list}, @{const union_list} and @{const diff_list} implement the corresponding
+set operations on lists. They are defined in Appendix~\ref{SetByList}. We have also replaced
 the set of productions @{const P} by a list @{const ps} and assume
 @{lemma "P = set (id ps)" by simp}.
 
@@ -547,13 +998,13 @@ Correctness and termination can be proved straightforwardly:
 assuming @{thm (prem 2) Close2s_if_Close2Ls}, @{thm (prem 3) Close2s_if_Close2Ls}
 (and in the second theorem @{thm (prem 3) Close2L_NF}).
 
-Note that the transition rules preserve the absence of duplicates in both \<open>B\<close> and \<open>C\<close>,
-but that this property is not needed in the above proofs.
-It will be needed in the later complexity analysis.
+%The transition rules preserve the absence of duplicates in both \<open>B\<close> and \<open>C\<close>,
+%but this property is not needed in the above proofs.
+%It will be needed in the later complexity analysis.
 
 \subsection{From Inductive to Recursive}
 
-Finally we take the step from inductive predicate to directly executable functional
+Now we take the step from inductive predicate to directly executable functional
 algorithm. We employ an Isabelle/HOL library theory defining a while-combinator
 \begin{quote}
 @{const_typ while_option}
@@ -585,24 +1036,25 @@ Correctness is provable by a standard invariant preservation argument:
 
 
 \subsection{Efficient Access to Bins}
+\label{sec:IL}
 
 The expensive part of the closure construction is checking, in each step,
 if a newly generated item is already present (in \<open>B\<close> or \<open>C\<close>).
 The number of possible items is bounded by the number of dotted productions (a constant
-\<open>k\<close> depending on @{const P}) times the number of possible @{const from} values,
-i.e.\ @{term "k * length w"}. We will store \<open>B\<close> and \<open>C\<close> not just as linear lists
-but will partition them by their @{const from} values. When searching for an item \<open>x\<close>,
+\<open>D\<close> depending on @{const P}) times the number of possible @{const from} values,
+i.e.\ @{term "D * length w"}. We will store \<open>B\<close> and \<open>C\<close> not just as linear lists
+but will pair them with a version partitioned by @{const from} values,
+i.e.\ as a list of lists indexed by @{const from} values. When searching for an item \<open>x\<close>,
 if we can access partition @{term "from x"} directly, the search takes
-time at most \<open>k\<close>, the maximum size of each partition.
+time at most \<open>D\<close>, the maximum size of each partition.
 When processing the \<open>i\<close>-th input character, i.e. @{term \<open>i = length Bs\<close>}, we
-augment \<open>B\<close> (and \<open>C\<close>) with a list (think array) \<open>F\<close> of size \<open>i\<close> such that
-@{term "F ! j"} is a list of all @{prop \<open>x \<in> B\<close>} where @{prop \<open>from x = j\<close>}.
-
+pair \<open>B\<close> (and \<open>C\<close>) with a list (think array) \<open>F\<close> of size \<open>i\<close> such that
+\mbox{@{term "F ! j"}} is a list of all @{prop \<open>x \<in> B\<close>} where @{prop \<open>from x = j\<close>}.
+The corresponding data type:
 \begin{quote}
-@{datatype [break] efficientItemList}
+@{datatype [break,margin=85] efficientItemList}
 \end{quote}
 with the projection functions @{const list} and @{const froms}.
-
 The invariant
 \begin{quote}
 @{thm [break] inv_IL.simps[of xs fs]}
@@ -629,14 +1081,22 @@ are defined in Appendix~\ref{SetByList2}.
 Finally, we are ready for the executable top-level algorithm,
 a refinement of @{const bins} from Section~\ref{sec:standard}:
 \begin{quote}
-@{thm [break,margin=85] bins_L.simps}\\
+@{thm [break,margin=85] bins_L.simps}\medskip
 
-@{thm Init_L_def}\\
+@{thm Init_L_def}\medskip
 
 @{thm [break] Scan_L_def}
 \end{quote}
+Note that at the end @{const close2_L} throws away the @{const froms} component
+and returns only the @{const list} which @{const bins_L} adds to \<open>Bs\<close>.
+The @{const froms} part is not useful any longer.
+(Except for the final search for an @{const is_final} item,
+but the improvement of that single step is marginal.)
 
-Correctness: @{thm bins_L_eq_\<S>}
+Correctness is expressed as in Section \ref{sec:standard}:
+\begin{quote}
+@{thm bins_L_eq_\<S>[OF _ le_refl]}
+\end{quote}
 \<close>
 text (in Earley_Gw_eps_T2)\<open>
 \section{Complexity}
@@ -653,21 +1113,193 @@ from Appendix~\ref{SetByList}) is defined like this:
 \end{quote}
 The boon and bane of this approach is that one obtains very detailed formulas with somewhat arbitrary
 constants. Arbitrary because they depend on the abstract machine model embodied in the generation of
-the time functions which may be quite different from a real machine.
+the time functions, which may be quite different from a real machine.
+As an extreme example, consider this upper bound:
 \begin{quote}
-@{thm [break] T_Scan_L_bound}
+@{thm [break] (sub) T_step_fun_bound}
 \end{quote}
-where @{const K} is the maximum length of the @{const rhs} of any production.
+Note the following:
+\begin{itemize}
+\item A large number of well-formedness assumptions are required, which we will elide in the rest
+of this section.
+\item In the upper bound term, @{const K} and @{const L} are constants depending on @{const ps}.
+\item
+Function @{term T_nth_IL} is a parameter of the analysis and assumed to be an upper bound of the
+real @{const T_nth}, and also of @{term T_list_update}, the time function for the list update
+function \<open>xs[i := x]\<close>.
+\end{itemize}
+There are two interesting choices for @{term T_nth_IL}:
+\begin{itemize}
+\item Linear time is the standard situation in functional programs.
+\item Constant time models array-like access and update of lists. We could achieve this
+by another refinement step using 
+Lammich's and Lochbihler's Collections library \cite{Collections-AFP,LammichL10} that offers
+imperative implementations of arrays with a purely functional, list-like interface
+specification.
+\end{itemize}
+Both choices are discussed below.
 
-@{thm [break] (concl) T_step_fun_bound}
 
-@{thm [break] T_step_fun_bound4[rename_abs _ il\<^sub>1 il\<^sub>2 _ il\<^sub>1 il\<^sub>2 _ il\<^sub>1 il\<^sub>2]}
+\subsection{Interlude: Asymptotic Complexity}
 
+In order to avoid such constant-studded upper bounds as shown above for @{const T_step_fun}
+we introduce a simple big $O$ framework, just enough for our purposes.
+In the following, \<open>f\<close> and \<open>g\<close> are of type @{typ "'a \<Rightarrow> nat"} and \<open>Q\<close> of type @{typ "'a \<Rightarrow> bool"}.
+\begin{quote}
+@{thm [break] le_O_def}
+\end{quote}
+The \<open>IF Q\<close> is dropped if \<open>Q\<close> is @{const True} everywhere.
+
+In contrast to the standard \<open>f \<in> O(g)\<close>, \<open>f\<close> and \<open>g\<close> are not defined on numbers but on an arbitrary type \<open>'a\<close>.
+For example, @{prop "(\<lambda>xs. 2 * length xs + 3) \<le> (\<lambda>xs. (length xs)^2)"} is true:
+take \<open>c = 1\<close> and \<open>d = 4\<close>. Our notation combines the measure function on some domain (here:
+the length of a list) with the growth function (here: linear and quadratic).
+It is easy to show that @{thm (prem 1) standard_BigO_if_le_O}, where  \<open>m ::\<close> @{typ "'a \<Rightarrow> nat"},
+implies the standard \<open>f \<in> O(g)\<close> under mild assumption (for example, that \<open>m\<close> is surjective
+and \<open>g\<close> is 0 only for finitely many arguments).
+
+In concrete instances, \<open>f\<close>, \<open>g\<close> and \<open>Q\<close> will be \<open>\<lambda>\<close> abstractions over the same parameter(s).
+Therefore we introduce a quantifier \isaconst{O} that shares the parameters:
+\begin{quote}
+@{thm [mode=fake_imp] BigO_iff_le_O}
+\end{quote}
+For example, the fictitious
+\begin{quote}
+@{prop "(\<lambda>(xs,i). T_f xs i) \<le>O (\<lambda>(xs,i). i) IF (\<lambda>(xs,i). i < length xs)"}
+\end{quote}
+becomes the more compact @{prop [mode=fake_imp]"BigO(\<lambda>(xs,i). (T_f xs i, i, i < length xs))"}
+
+
+\subsection{Earley Complexity}
+
+We have analyzed the complexity of our Earley recognizer with all constants present
+and in terms of an upper bound @{term T_nth_IL} for @{const T_nth}.
+We present the result at the end of this section.
+For readability the running times of selected auxiliary functions
+are presented in \isaconst{O} notation.
+Except in the final result,
+\emph{we assume @{term T_nth_IL} is constant and we drop all preconditions for readability}.
+%\emph{Distinctness of productions (@{prop "distinct ps"}) is a global assumption in this section.}
+
+Because of the constant time @{const nth} assumption,
+single element set operations are constant time as well
+\begin{quote}
+@{thm [mode=no_fake_imp] T_isin_O[rename_abs il x]}\medskip
+
+@{thm [mode=no_fake_imp] T_insert_O[rename_abs x il]}
+\end{quote}
+while combinations of sets take linear time:
+\begin{quote}
+@{thm [mode=no_fake_imp] T_union_LIL_wf5[rename_abs xs il]}\medskip
+
+@{thm [mode=no_fake_imp] T_minus_IL_wf5[rename_abs il\<^sub>1 il\<^sub>2]}
+\end{quote}
+
+Each evaluation of @{const step_fun} requires a (constant) number of set operations
+that are all of either constant time or linear time in @{term "length Bs"}.
+Moreover, @{const Predict_L} is obviously constant time (because @{const ps} is fixed).
+Evaluation of @{term "Complete_L Bs x"} is linear in @{term "Bs!from x"},
+which is linear in @{term "length Bs"}.
+Hence the overall complexity of @{const step_fun} is also linear in @{term "length Bs"}:
+\begin{quote}
+@{thm [mode=no_fake_imp] T_step_fun_bound_O[rename_abs Bs il\<^sub>1 il\<^sub>2]}
+\end{quote}
+
+Now we need to analyze the complexity of @{const close2_L}, which is defined by means of
+@{const while_option}. However,
+the infrastructure for generation of running time functions is restricted to total functions
+(although they may be undefined for particular argument patterns).
+Therefore we have to set up @{const T_while_option} by hand. We simply add an accumulator
+that counts the computation steps:
+\begin{quote}
+@{thm T_while_option2_def[of _ _ tf]}
+\end{quote}
+In the end we project on the counter:
+\begin{quote}
+@{thm T_while_option_def[of _ _ tf]}
+\end{quote}
+Now we can define the time function for @{const close2_L}:
+\begin{quote}
+@{thm [break] (sub) T_close2_IL_def}
+\end{quote}
+At the beginning of Section \ref{sec:IL} we explained that there are at most @{term "D * length w"}
+well-formed items. More precisely, when processing input symbol number @{term "length Bs"},
+there are @{term "D * (length Bs+1)"} well-formed items.
+Because each iteration of @{const close2_L}~\<open>Bs\<close> takes time proportional to @{term "length Bs"}
+and adds at least one item (or shifts one item from \<open>B\<close> to \<open>C\<close>), the execution of @{const close2_L}
+has quadratic complexity:
+\begin{quote}
+@{thm [mode=no_fake_imp] T_close2_IL_O[rename_abs Bs il\<^sub>1 il\<^sub>2]}
+\end{quote}
+Because each closure takes quadratic time and @{const bins_L} performs linearly many closure steps,
+its overall complexity is cubic:
+\begin{quote}
+@{thm [mode=fake_imp] T_bins_IL_O[rename_abs k]}
+\end{quote}
+
+Because @{const accepted} (see Section \ref{sec:EarleyInductive})
+requires a single scan of the last bin (to search for an @{const is_final} item),
+and its size is bounded by @{term "D*length w"},
+the time to compute @{const accepted} @{term w} is bounded by @{term "T_bins_L (length w) + D*length w"}
+and is thus cubic in @{term "length w"}.
+This confirms Earley's informal analysis.
+
+The above big \isaconst{O} complexities are simplified versions of the more precise
+bounds we proved. We close this section with the upper bound
+we proved for our full recognizer. We spare the reader the definition of the constants:
+\begin{quote}
+@{term "C\<^sub>1 *((length w)+2)^3 + C\<^sub>2 * ((length w)+2)^3 * T_nth_IL ((length w)+1)"}
+\end{quote}
+Note that this bound is a function of @{term T_nth_IL}. It tells us that if @{const nth}
+takes linear time (as opposed to constant time as assumed above), our recognizer
+has quartic complexity. This confirms the informal analysis by Rau and Nipkow \cite{RauN24}.
+
+
+\section{Conclusion}
+
+We have completed the development of a verified executable Earley recognizer started by Nipkow and Rau.
+In particular, we have verified its complexity. We have also verified an Earley parser for unambiguous grammars
+(with the same asymptotic complexity as the recognizer), but its presentation would go beyond the scope
+of the current paper.
+
+This is work in progress. The following points, in increasing order of difficulty,
+need to be addressed in the future:
+\begin{itemize}
+\item Lists indexed by @{const from} values should be implemented by proper arrays from
+the Isabelle Collections framework \cite{Collections-AFP,LammichL10}.
+\item The restriction to epsilon-free grammars should be lifted.
+\item The Big \isaconst{O} framework needs to be automated. In particular, it should
+  support deriving big \isaconst{O} complexities directly, without having to
+  derive precise bounds first.
+\item The parser (not presented in this paper) should be generalized from unambiguous to arbitrary
+grammars.
+\end{itemize}
+
+\begin{credits}
+\subsubsection{\ackname}
+The first author would like to thank Larry Paulson for inventing the Isabelle theorem prover
+and for employing him many years ago to work on the further development of Isabelle.
+It was a profound and happy change of direction.
+
+%\vspace{-1ex}
+\subsubsection{\discintname}
+%It is now necessary to declare any competing interests or to specifically
+%state that the authors have no competing interests. Please place the
+%statement with a bold run-in heading in small font size beneath the
+%(optional) acknowledgments
+%for example:
+The authors have no competing interests to declare that are relevant to the content of this article.
+\end{credits}
+
+\bibliographystyle{splncs04}
+\bibliography{root}
 
 \appendix
 
 \section{Set Operations on type  @{type list}}
 \label{SetByList}
+
+The definitions in this and the next appendix are mostly self-explanatory.
 
 \begin{quote}
 @{thm filter.simps}\\
@@ -686,11 +1318,10 @@ where @{const K} is the maximum length of the @{const rhs} of any production.
 \section{Set Operations on type @{type efficientItemList}}
 \label{SetByList2}
 
-The following definitions are mostly self-explanatory.
 \begin{quote}
 @{thm [break] EarleyWorklist.isin.simps}\\
 
-@{thm [break] empty_IL_def}\\
+@{thm [break] empty_IL_def[unfolded empty_froms_is_replicate]}\\
 
 @{thm [break] insert.simps}\\
 
